Update word_removeProof
It is actually mostly rewritten, trying a different style.
With Yong Kiam (towards the end).

compiler/backend/proofs/word_removeProofScript.sml
@@ -2,180 +2,280 @@ open preamble word_removeTheory wordSemTheory wordPropsTheory;
 
 val _ = new_theory "word_removeProof";
 
-(* semantics *)
-val alloc_termdep_code_frame = Q.prove(`
-  alloc c names (s with <|termdep:=d;code:=l|>) =
-  (FST (alloc c names s),SND(alloc c names s) with <|termdep:=d;code:=l|>)`,
-  full_simp_tac(srw_ss())[alloc_def]>>TOP_CASE_TAC>>
-  full_simp_tac(srw_ss())[push_env_def,env_to_list_def,LET_THM,gc_def,set_store_def]>>
-  ntac 3(FULL_CASE_TAC>>full_simp_tac(srw_ss())[])
-  >-
-    (EVERY_CASE_TAC>>full_simp_tac(srw_ss())[])>>
-  FULL_CASE_TAC>>full_simp_tac(srw_ss())[pop_env_def]>>
-  ntac 3(FULL_CASE_TAC>>full_simp_tac(srw_ss())[call_env_def])>>
-  FULL_CASE_TAC>>full_simp_tac(srw_ss())[has_space_def]>>
-  EVERY_CASE_TAC>>full_simp_tac(srw_ss())[])|>INST_TYPE[beta|->alpha,gamma|->beta,delta|->alpha]
+(* TODO : move *)
+val map_union = Q.store_thm("map_union",
+  `∀t1 t2. map f (union t1 t2) = union (map f t1) (map f t2)`,
+  Induct
+  \\ rw[map_def,union_def]
+  \\ TOP_CASE_TAC
+  \\ rw[map_def,union_def]);
+(* -- *)
 
-val get_vars_termdep_code_frame = Q.prove(`
-  ∀ls.
-  get_vars ls s = get_vars ls (s with <|termdep:=0;code:=l|>)`,
-  Induct>>full_simp_tac(srw_ss())[get_vars_def,get_var_def])
+val compile_state_def = Define`
+  compile_state clk c s =
+    s with <|
+      clock := s.clock+clk;
+      termdep := 0;
+      code := map (I ## remove_must_terminate) s.code;
+      compile_oracle := (I ## (MAP (I ## I ## remove_must_terminate))) o s.compile_oracle;
+      compile := c
+    |>`;
 
-val word_exp_termdep_code_frame = Q.prove(`
-  ∀s exp.
-  word_exp s exp = word_exp (s with <|termdep:=0;code:=l|>) exp`,
-  ho_match_mp_tac word_exp_ind>>
-  full_simp_tac(srw_ss())[word_exp_def,LET_THM,mem_load_def]>>
-  full_simp_tac(srw_ss())[EVERY_MAP,EVERY_MEM]>>srw_tac[][]>>
-  AP_THM_TAC >> AP_THM_TAC >>
-  AP_TERM_TAC>> AP_TERM_TAC>>
-  full_simp_tac(srw_ss())[MAP_EQ_f])
+val compile_state_const = Q.store_thm("compile_state_const[simp]",
+  `(compile_state clk c s).locals = s.locals ∧
+   (compile_state clk c s).permute = s.permute ∧
+   (compile_state clk c s).ffi = s.ffi ∧
+   (compile_state clk c s).code_buffer = s.code_buffer ∧
+   (compile_state clk c s).data_buffer = s.data_buffer ∧
+   (compile_state clk c s).code = map (I ## remove_must_terminate) s.code ∧
+   (compile_state clk c s).clock = s.clock + clk ∧
+   (compile_state clk c s).termdep = 0 ∧
+   (compile_state clk c s).compile_oracle = (I ## (MAP (I ## I ## remove_must_terminate))) o s.compile_oracle ∧
+   (compile_state clk c s).compile = c ∧
+   (compile_state clk c s).stack = s.stack ∧
+   (compile_state clk c s).store = s.store ∧
+   (compile_state clk c s).memory = s.memory ∧
+   (compile_state clk c s).mdomain = s.mdomain ∧
+   (compile_state clk c s).be = s.be ∧
+   (compile_state clk c s).gc_fun = s.gc_fun ∧
+   (compile_state clk c s).handler = s.handler`,
+  EVAL_TAC);
 
-val tac = (full_simp_tac(srw_ss())[GSYM word_exp_termdep_code_frame]>>EVERY_CASE_TAC>>full_simp_tac(srw_ss())[state_component_equality,set_store_def,mem_store_def])
+val find_code_map_I = Q.store_thm("find_code_map_I[simp]",
+  `find_code d l (map (I ## f) t) = OPTION_MAP (I ## f) (find_code d l t)`,
+  Cases_on`d` \\ rw[find_code_def,lookup_map]
+  \\ rpt(TOP_CASE_TAC \\ fs[]));
 
-val push_env_code = Q.prove(`
-  (push_env x handler s).code = s.code`,
-  Cases_on`handler`>>TRY(PairCases_on`x'`)>>full_simp_tac(srw_ss())[push_env_def,LET_THM,env_to_list_def])
+val compile_state_update = Q.store_thm("compile_state_update[simp]",
+  `compile_state clk c s with stack updated_by f1 = compile_state clk c (s with stack updated_by f1) ∧
+   compile_state clk c s with permute updated_by f2 = compile_state clk c (s with permute updated_by f2) ∧
+   compile_state clk c s with ffi updated_by f10 = compile_state clk c (s with ffi updated_by f10) ∧
+   compile_state clk c s with data_buffer updated_by f9 = compile_state clk c (s with data_buffer updated_by f9) ∧
+   compile_state clk c s with code_buffer updated_by f8 = compile_state clk c (s with code_buffer updated_by f8) ∧
+   compile_state clk c s with memory updated_by f7 = compile_state clk c (s with memory updated_by f7) ∧
+   compile_state clk c s with locals updated_by f6 = compile_state clk c (s with locals updated_by f6) ∧
+   compile_state clk c s with memory updated_by f5 = compile_state clk c (s with memory updated_by f5) ∧
+   compile_state clk c s with store updated_by f4 = compile_state clk c (s with store updated_by f4) ∧
+   compile_state clk c s with handler updated_by f3 = compile_state clk c (s with handler updated_by f3)`,
+  EVAL_TAC);
 
-val pop_env_termdep_code_frame = Q.prove(`
-  pop_env (r' with <|termdep:=0; code:=l|>) =
-  lift (λs. s with <|termdep:=0;code:=l|>) (pop_env r')`,
-  full_simp_tac(srw_ss())[pop_env_def]>>EVERY_CASE_TAC>>full_simp_tac(srw_ss())[])
+val get_var_compile_state = Q.store_thm("get_var_compile_state[simp]",
+  `get_var x (compile_state clk c s) = get_var x s`,
+  EVAL_TAC);
 
-val word_remove_correct = Q.store_thm("word_remove_correct",`
-  ∀prog st res rst.
-  (!n v p. lookup n st.code = SOME (v,p) ==>
-         lookup n l = SOME (v,remove_must_terminate p)) ∧
-  evaluate(prog,st) = (res,rst) ∧
-  res ≠ SOME Error ⇒
-  ∃clk.
-  evaluate(remove_must_terminate prog,st with <|clock:=st.clock+clk;termdep:=0;code:=l|>) = (res,rst with <|termdep:=0;code:=l|>)`,
-  recInduct evaluate_ind>>
-  full_simp_tac(srw_ss())[evaluate_def,remove_must_terminate_def,state_component_equality,call_env_def,get_var_def,set_var_def,dec_clock_def]>>srw_tac[][]
-  >-
-    (EVERY_CASE_TAC>>full_simp_tac(srw_ss())[]>>
-    imp_res_tac alloc_const>>
-    simp[alloc_termdep_code_frame,state_component_equality])
-  >-
-    (simp[GSYM get_vars_termdep_code_frame]>>
-    EVERY_CASE_TAC>>
-    full_simp_tac(srw_ss())[set_vars_def,state_component_equality]>>rev_full_simp_tac(srw_ss())[])
-  >-
-    (Cases_on`i`>>full_simp_tac(srw_ss())[inst_def,state_component_equality,assign_def,GSYM word_exp_termdep_code_frame,get_var_def,GSYM get_vars_termdep_code_frame,LET_THM]>>
-    rpt(TOP_CASE_TAC>>full_simp_tac(srw_ss())[set_var_def,state_component_equality,mem_load_def,get_var_def,mem_store_def]))
-  >- tac
-  >- tac
-  >- tac
-  >- (tac>>FULL_CASE_TAC>>full_simp_tac(srw_ss())[state_component_equality])
-  >- (qexists_tac`0`>>simp[state_component_equality])
-  >- (qexists_tac`0`>>simp[state_component_equality])
-  >- (*hard*)
-    (qpat_x_assum`A=(res,rst)`mp_tac>>simp[]>>
-    pairarg_tac>>full_simp_tac(srw_ss())[]>>
-    IF_CASES_TAC>>full_simp_tac(srw_ss())[]>>
-    strip_tac>>full_simp_tac(srw_ss())[]>>
-    rveq>>
-    res_tac>>
-    imp_res_tac evaluate_dec_clock>>full_simp_tac(srw_ss())[]>>
-    imp_res_tac evaluate_add_clock>>full_simp_tac(srw_ss())[]>>
-    pop_assum kall_tac>>
-    first_x_assum(qspec_then`s.clock` assume_tac)>>
-    metis_tac[])
-  >-
-    (qpat_x_assum`A=(res,rst)`mp_tac>>simp[]>>
-    pairarg_tac>>full_simp_tac(srw_ss())[]>>
-    IF_CASES_TAC>>full_simp_tac(srw_ss())[]>-
-      (strip_tac>>full_simp_tac(srw_ss())[]>>
-      imp_res_tac evaluate_consts>>
-      full_simp_tac(srw_ss())[]>>
-      imp_res_tac evaluate_add_clock>>
-      rev_full_simp_tac(srw_ss())[]>>pop_assum kall_tac>>
-      qexists_tac`clk+clk'`>>ntac 2 strip_tac>>
-      pop_assum(qspec_then`clk'` assume_tac)>>full_simp_tac(srw_ss())[ADD_COMM]>>
-      `s.clock + (clk+clk') = clk'+(clk+s.clock)` by simp[]>>
-      full_simp_tac(srw_ss())[]>>srw_tac[][]>>
-      simp[])
-    >>
-      srw_tac[][]>>full_simp_tac(srw_ss())[]>>
-      qexists_tac`clk`>>full_simp_tac(srw_ss())[ADD_COMM])
-  >- tac
-  >- (tac>>full_simp_tac(srw_ss())[jump_exc_def]>>tac)
-  >-
-    (Cases_on`ri`>>full_simp_tac(srw_ss())[get_var_imm_def,get_var_def]>>
-    ntac 5(TOP_CASE_TAC>>full_simp_tac(srw_ss())[]))
-  >-
-    (fs[domain_lookup,EXISTS_PROD] \\ res_tac \\ fs[]
-     \\ fs[state_component_equality] )
-  >- (
-     ntac 6(TOP_CASE_TAC>>full_simp_tac(srw_ss())[])>>
-    full_simp_tac(srw_ss())[LET_THM]>>pairarg_tac>>full_simp_tac(srw_ss())[state_component_equality]>>
-    rveq>>full_simp_tac(srw_ss())[])
-  >>
-    simp[markerTheory.Abbrev_def]>>
-    qpat_x_assum`A=(res,rst)` mp_tac>>
-    simp[evaluate_def,GSYM get_vars_termdep_code_frame]>>
-    TOP_CASE_TAC>>full_simp_tac(srw_ss())[]>>
-    TOP_CASE_TAC>>full_simp_tac(srw_ss())[]>>
-    TOP_CASE_TAC>>full_simp_tac(srw_ss())[]>>
-    TOP_CASE_TAC>>full_simp_tac(srw_ss())[]>>
-    qpat_abbrev_tac `newprog = find_code dest aret l`>>
-    `newprog = SOME (q,remove_must_terminate r)` by
-      (Cases_on`ret`>>Cases_on`dest`>>
-      unabbrev_all_tac>>full_simp_tac(srw_ss())[find_code_def,add_ret_loc_def]>>
-      EVERY_CASE_TAC>>full_simp_tac(srw_ss())[add_ret_loc_def]>>
-      res_tac>>
-      rveq>>full_simp_tac(srw_ss())[]>>
-      metis_tac[NOT_NONE_SOME])>>
-    simp[]>>
-    TOP_CASE_TAC>-
-      (TOP_CASE_TAC>>full_simp_tac(srw_ss())[]>>
-      TOP_CASE_TAC>>full_simp_tac(srw_ss())[]
-      >-
-        (strip_tac>>qexists_tac`0`>>full_simp_tac(srw_ss())[call_env_def,state_component_equality])
-      >>
-      EVERY_CASE_TAC>>srw_tac[][]>>
-      first_x_assum(qspecl_then[`SOME x'`,`r'`] assume_tac)>>rev_full_simp_tac(srw_ss())[]>>
-      qexists_tac`clk`>>simp[dec_clock_def,call_env_def]>>
-      `clk + s.clock -1 = s.clock -1 + clk` by DECIDE_TAC>>
-      full_simp_tac(srw_ss())[])>>
-    ntac 7 (TOP_CASE_TAC>>full_simp_tac(srw_ss())[])>-
-      (srw_tac[][]>>qexists_tac`0`>>full_simp_tac(srw_ss())[call_env_def,state_component_equality])>>
-    ntac 3 (TOP_CASE_TAC>>full_simp_tac(srw_ss())[])
-    >-
-      (ntac 3 (TOP_CASE_TAC>>full_simp_tac(srw_ss())[])>>
-      Cases_on`handler`>>TRY(PairCases_on`x'''`)>>full_simp_tac(srw_ss())[push_env_def,LET_THM,env_to_list_def,dec_clock_def,call_env_def]>>rev_full_simp_tac(srw_ss())[]>>srw_tac[][]>>
-      imp_res_tac evaluate_consts>>
-      imp_res_tac pop_env_code_gc_fun_clock>>
-      full_simp_tac(srw_ss())[]>>rev_full_simp_tac(srw_ss())[]>>
-      qexists_tac`clk+clk'`>>
-      imp_res_tac evaluate_add_clock>>
-      full_simp_tac(srw_ss())[]>>
-      pop_assum kall_tac>>
-      pop_assum (qspec_then`clk'` mp_tac)>>simp[]>>
-      full_simp_tac(srw_ss())[pop_env_termdep_code_frame,set_var_def]>>
-      full_simp_tac(srw_ss())[ADD_COMM])
-    >-
-      (Cases_on`handler`>>TRY(PairCases_on`x''`)>>full_simp_tac(srw_ss())[push_env_def,LET_THM,env_to_list_def,dec_clock_def,call_env_def]>>rev_full_simp_tac(srw_ss())[]
-      >-
-        (srw_tac[][]>>qexists_tac`clk`>>
-        `s.clock -1 + clk = clk + s.clock-1`by DECIDE_TAC>>
-        rveq>>full_simp_tac(srw_ss())[])
-      >>
-        ntac 2 (TOP_CASE_TAC>>full_simp_tac(srw_ss())[])>>srw_tac[][]>>
-        imp_res_tac evaluate_consts>>
-        imp_res_tac pop_env_code_gc_fun_clock>>
-        full_simp_tac(srw_ss())[]>>rev_full_simp_tac(srw_ss())[]>>
-        qexists_tac`clk+clk'`>>
-        imp_res_tac evaluate_add_clock>>
-        full_simp_tac(srw_ss())[]>>
-        ntac 2 (pop_assum kall_tac)>>
-        pop_assum (qspec_then`clk'` mp_tac)>>simp[]>>
-        full_simp_tac(srw_ss())[ADD_COMM,set_var_def])
-    >>
-      Cases_on`handler`>>TRY(PairCases_on`x''`)>>full_simp_tac(srw_ss())[push_env_def,LET_THM,env_to_list_def,dec_clock_def,call_env_def]>>rev_full_simp_tac(srw_ss())[]>>strip_tac>>
-      qexists_tac`clk`>>
-      `s.clock -1 + clk = clk + s.clock-1`by DECIDE_TAC>>
-      rveq>>full_simp_tac(srw_ss())[])
+val get_vars_compile_state = Q.store_thm("get_vars_compile_state[simp]",
+  `∀xs s. get_vars xs (compile_state clk c s) = get_vars xs s`,
+  Induct \\ rw[get_vars_def]);
+
+val set_var_compile_state = Q.store_thm("set_var_compile_state[simp]",
+  `set_var x y (compile_state clk c s) = compile_state clk c (set_var x y s)`,
+  rw[set_var_def]);
+
+val set_vars_compile_state = Q.store_thm("set_vars_compile_state[simp]",
+  `set_vars xs ys (compile_state clk c s) = compile_state clk c (set_vars xs ys s)`,
+  EVAL_TAC);
+
+val set_store_compile_state = Q.store_thm("set_store_compile_state[simp]",
+  `set_store x y (compile_state clk c s) = compile_state clk c (set_store x y s)`,
+  EVAL_TAC);
+
+val push_env_compile_state = Q.store_thm("push_env_compile_state[simp]",
+  `push_env env h (compile_state clk c s) = compile_state clk c (push_env env h s)`,
+  Cases_on`h` \\ TRY(PairCases_on`x`) \\ rw[push_env_def,UNCURRY]);
+
+val pop_env_compile_state = Q.store_thm("pop_env_compile_state[simp]",
+  `pop_env (compile_state clk c s) = OPTION_MAP (compile_state clk c) (pop_env s)`,
+  rw[pop_env_def] \\ ntac 4 (CASE_TAC \\ fs[]));
+
+val call_env_compile_state = Q.store_thm("call_env_compile_state[simp]",
+  `call_env x (compile_state clk c z) = compile_state clk c (call_env x z)`,
+  EVAL_TAC);
+
+val has_space_compile_state = Q.store_thm("has_space_compile_state[simp]",
+  `has_space n (compile_state clk c s) = has_space n s`,
+  EVAL_TAC);
+
+val gc_compile_state = Q.store_thm("gc_compile_state[simp]",
+  `gc (compile_state clk c s) = OPTION_MAP (compile_state clk c) (gc s)`,
+  rw[gc_def] \\ ntac 4 (CASE_TAC \\ simp[]));
+
+val alloc_compile_state = Q.store_thm("alloc_compile_state[simp]",
+  `alloc w names (compile_state clk c s) = (I ## compile_state clk c) (alloc w names s)`,
+  rw[alloc_def] \\ ntac 6 (CASE_TAC \\ fs[]));
+
+val mem_load_compile_state = Q.store_thm("mem_load_compile_state[simp]",
+  `mem_load w (compile_state clk c s) = mem_load w s`,
+  EVAL_TAC);
+
+val mem_store_compile_state = Q.store_thm("mem_store_compile_state[simp]",
+  `mem_store x y (compile_state clk c s) = OPTION_MAP (compile_state clk c) (mem_store x y s)`,
+  rw[mem_store_def]);
+
+val word_exp_compile_state = Q.store_thm("word_exp_compile_state[simp]",
+  `∀s y.  word_exp (compile_state clk c s) y = word_exp s y`,
+  recInduct word_exp_ind
+  \\ rw[word_exp_def]
+  \\ fsrw_tac[ETA_ss][]
+  \\ `MAP (word_exp (compile_state clk c s)) wexps = MAP (word_exp s) wexps`
+  by fs[MAP_EQ_f] \\ fs[]);
+
+val assign_compile_state = Q.store_thm("assign_compile_state[simp]",
+  `assign x y (compile_state clk c s) = OPTION_MAP (compile_state clk c) (assign x y s)`,
+  rw[assign_def] \\ CASE_TAC \\ fs[]);
+
+val inst_compile_state = Q.store_thm("inst_compile_state[simp]",
+  `inst i (compile_state clk c s) = OPTION_MAP (compile_state clk c) (inst i s)`,
+  rw[inst_def] \\ rpt(TOP_CASE_TAC \\ fs[]) \\ fs[]);
+
+val compile_state_dec_clock = Q.store_thm("compile_state_dec_clock[simp]",
+  `s.clock ≠ 0 ⇒ (compile_state clk c (dec_clock s) = dec_clock (compile_state clk c s))`,
+  EVAL_TAC \\ rw[state_component_equality]);
+
+val jump_exc_compile_state = Q.store_thm("jump_exc_compile_state[simp]",
+  `jump_exc (compile_state clk c s) = OPTION_MAP (compile_state clk c ## I) (jump_exc s)`,
+  rw[jump_exc_def] \\ ntac 5 (CASE_TAC \\ fs[]));
+
+val get_var_imm_compile_state = Q.store_thm("get_var_imm_compile_state[simp]",
+  `get_var_imm x (compile_state clk c s) = get_var_imm x s`,
+  Cases_on`x` \\ rw[get_var_imm_def]);
+
+val push_env_case_handler = Q.store_thm("push_env_case_handler[simp]",
+  `push_env x (case handler of NONE => NONE | SOME (v,prog,l1,l2) => SOME (v, f prog, l1,l2)) = push_env x handler`,
+  CASE_TAC \\ rw[push_env_def]
+  \\ split_pair_case_tac \\ rw[push_env_def,FUN_EQ_THM]);
+
+val word_remove_correct = Q.store_thm("word_remove_correct",
+  `∀prog st res rst.
+    evaluate (prog,st) = (res,rst) ∧
+    st.compile = (λcfg. c cfg o (MAP (I ## I ## remove_must_terminate))) ∧
+    res ≠ SOME Error ⇒
+    ∃clk.
+      evaluate (remove_must_terminate prog, compile_state clk c st) =
+        (res, compile_state 0 c rst)`,
+  recInduct evaluate_ind
+  \\ rw[evaluate_def,remove_must_terminate_def]
+  \\ TRY ( (* Seq *)
+    qmatch_goalsub_rename_tac`remove_must_terminate _` \\
+    pairarg_tac \\ fs[] \\
+    reverse(fs[case_eq_thms] \\ rveq \\ fs[])
+    >- ( qexists_tac`clk` \\ fs[] \\ NO_TAC ) \\
+    qpat_x_assum`(res,rst) = _`(assume_tac o SYM) \\ fs[] \\
+    `s1.compile = s.compile` by (imp_res_tac evaluate_consts \\ fs[]) \\ fs[] \\
+    qexists_tac`clk + clk'` \\ fs[] \\
+    imp_res_tac (GEN_ALL evaluate_add_clock) \\ fs[] \\
+    first_x_assum(qspec_then`clk'`mp_tac) \\ fs[] \\
+    fs[compile_state_def] \\ NO_TAC )
+  \\ TRY ( (* MustTerminate *)
+    qmatch_goalsub_rename_tac`remove_must_terminate _` \\
+    pairarg_tac \\ fs[] \\
+    fs[case_eq_thms] \\ rveq \\ fs[] \\
+    qpat_x_assum`evaluate(p,_) = _`kall_tac \\
+    drule evaluate_dec_clock \\ fs[] \\ strip_tac \\
+    drule (GEN_ALL evaluate_add_clock) \\ fs[] \\
+    disch_then(qspec_then`s.clock`mp_tac) \\
+    strip_tac \\
+    fs[compile_state_def] \\
+    qexists_tac`clk + MustTerminate_limit (:'a) - s1.clock` \\
+    fs[] \\ NO_TAC)
+  \\ TRY ( (* Install *)
+    fs[case_eq_thms] \\ rveq \\
+    pairarg_tac \\ fs[] \\
+    pairarg_tac \\ fs[] \\
+    fs[case_eq_thms] \\ rveq \\ fs[] \\
+    fs[shift_seq_def] \\
+    qexists_tac`0` \\
+    simp[compile_state_def,state_component_equality,FUN_EQ_THM,map_union,map_fromAList] \\
+    rpt(AP_TERM_TAC ORELSE AP_THM_TAC) \\ simp[FUN_EQ_THM,FORALL_PROD] \\ NO_TAC)
+  \\ TRY ( (* Call *)
+    qmatch_goalsub_rename_tac`find_code` \\
+    TOP_CASE_TAC \\ fs[] \\
+    TOP_CASE_TAC \\ fs[] \\
+    qpat_x_assum`_ = (res,rst)`mp_tac \\
+    TOP_CASE_TAC \\ fs[] \\
+    TOP_CASE_TAC \\ fs[] \\
+    TOP_CASE_TAC \\ fs[]
+    >- (
+      fs[case_eq_thms] \\
+      strip_tac \\ fs[] \\ rveq
+      >- metis_tac[]
+      \\ rfs[]
+      \\ fs[compile_state_def,dec_clock_def,call_env_def]
+      \\ qexists_tac`clk` \\ fs[] )
+    \\ split_pair_case_tac \\ fs[] \\
+    TOP_CASE_TAC \\ fs[] \\
+    TOP_CASE_TAC \\ fs[] \\
+    TOP_CASE_TAC \\ fs[]
+    >- (
+      strip_tac \\ rveq \\ fs[] \\
+      qexists_tac`0` \\ fs[] \\
+      fs[add_ret_loc_def] ) \\
+    fs[add_ret_loc_def] \\
+    TOP_CASE_TAC \\ fs[] \\
+    TOP_CASE_TAC \\ fs[] \\
+    rfs[] \\
+    TOP_CASE_TAC \\ fs[] \\ rveq \\
+    simp[Once case_eq_thms]
+    >- (
+      simp[Once case_eq_thms]
+      \\ strip_tac \\ fs[]
+      \\ rveq \\ fs[]
+      \\ pop_assum mp_tac
+      \\ IF_CASES_TAC \\ fs[]
+      \\ strip_tac \\ fs[] \\ rfs[]
+      \\ imp_res_tac pop_env_const
+      \\ imp_res_tac evaluate_consts \\ fs[] \\ rfs[]
+      \\ qexists_tac`clk + clk'`
+      \\ imp_res_tac evaluate_add_clock \\ fs[]
+      \\ pop_assum kall_tac
+      \\ first_x_assum(qspec_then`clk'`mp_tac)
+      \\ qmatch_goalsub_abbrev_tac`remove_must_terminate _,sa`
+      \\ strip_tac
+      \\ qmatch_goalsub_abbrev_tac`remove_must_terminate _,sb`
+      \\ `sa = sb` by (
+        unabbrev_all_tac
+        \\ simp[dec_clock_def]
+        \\ simp[state_component_equality] )
+      \\ rw[]
+      \\ fs[compile_state_def] )
+    >- (
+      strip_tac \\ fs[] \\ rveq \\ fs[]
+      >- (
+        fs[dec_clock_def]
+        \\ qexists_tac`clk` \\ fs[]
+        \\ qmatch_goalsub_abbrev_tac`remove_must_terminate _,sa`
+        \\ qmatch_asmsub_abbrev_tac`remove_must_terminate _,sb`
+        \\ `sa = sb` by ( unabbrev_all_tac \\ simp[state_component_equality] )
+        \\ rw[] )
+      \\ split_pair_case_tac \\ fs[] \\ rveq \\ fs[]
+      \\ pop_assum mp_tac \\ simp[Once case_eq_thms]
+      \\ simp[Once case_eq_thms]
+      \\ strip_tac \\ rveq \\ fs[]
+      \\ pop_assum(assume_tac o SYM) \\ fs[]
+      \\ imp_res_tac evaluate_consts \\ fs[] \\ rfs[]
+      \\ qexists_tac`clk + clk'`
+      \\ imp_res_tac evaluate_add_clock \\ fs[]
+      \\ pop_assum kall_tac
+      \\ first_x_assum(qspec_then`clk'`mp_tac)
+      \\ qmatch_goalsub_abbrev_tac`remove_must_terminate _,sa`
+      \\ strip_tac
+      \\ qmatch_goalsub_abbrev_tac`remove_must_terminate _,sb`
+      \\ `sa = sb` by (
+        unabbrev_all_tac
+        \\ simp[dec_clock_def]
+        \\ simp[state_component_equality] )
+      \\ rw[]
+      \\ fs[compile_state_def] )
+    \\ strip_tac \\ rveq \\ fs[]
+    \\ fs[dec_clock_def]
+    \\ qexists_tac`clk` \\ fs[]
+    \\ qmatch_goalsub_abbrev_tac`remove_must_terminate _,sa`
+    \\ qmatch_asmsub_abbrev_tac`remove_must_terminate _,sb`
+    \\ `sa = sb` by ( unabbrev_all_tac \\ simp[state_component_equality] )
+    \\ rw[] \\ NO_TAC )
+  \\ fs[case_eq_thms] \\ rveq
+  \\ fs[domain_map]
+  \\ rpt(pairarg_tac \\ fs[])
+  \\ metis_tac[]);
 
 (* syntactic preservation all in one go *)
 val convs = [flat_exp_conventions_def,full_inst_ok_less_def,every_inst_def,post_alloc_conventions_def,call_arg_convention_def,wordLangTheory.every_stack_var_def,wordLangTheory.every_var_def,extract_labels_def]
